theories/acyclic_wf.v
@@ -1,0 +1,41 @@
+From stdpp Require Import relations finite.
+From Coq Require Import ssreflect.
+
+Section acyclic_wf.
+  Context {A : Type} (R : relation A).
+
+  Lemma tc_refl_ex_loop x :
+    tc R x x → ex_loop R x.
+  Proof.
+    intros HR. apply ex_loop_tc. cofix IH. econstructor; eauto.
+  Qed.
+
+  Lemma tc_flip x y :
+    tc (flip R) x y → tc R y x.
+  Proof.
+    induction 1.
+    - by apply tc_once.
+    - eapply tc_r; eauto. 
+  Qed.
+
+  Definition acyclic (R : relation A) : Prop := ∀ x, ¬ ex_loop R x.
+
+  Context `{Finite A}.
+
+  Lemma acyclic_flip_wf :
+    acyclic R → wf (flip R).
+  Proof.
+    intros Hno x. apply tc_finite_sn.
+    - intros y Htc. eapply Hno. apply tc_refl_ex_loop; eauto.
+    - unfold pred_finite. eexists => ? ?. apply elem_of_enum.
+  Qed.
+
+  Lemma acyclic_wf :
+    acyclic R → wf R.
+  Proof.
+    intros Hno x. apply tc_finite_sn.
+    - intros y Htc. eapply Hno. apply tc_refl_ex_loop, tc_flip; eauto.
+    - unfold pred_finite. eexists => ? ?. apply elem_of_enum.
+  Qed.
+
+End acyclic_wf.
