theories/encoding.v
@@ -1,10 +1,10 @@
-From stdpp Require Import prelude sorting.
+From stdpp Require Import prelude sorting finite.
 From Coq Require Import ssreflect.
 From ambig Require Import grammar util ambiguity acyclic sub_derive slice derivation witness.
 
 Section encoding.
 
-  Context {Σ N : Type} `{EqDecision Σ} `{Inhabited Σ} `{EqDecision N}.
+  Context {Σ N : Type} `{EqDecision Σ} `{Inhabited Σ} `{EqDecision N} `{Finite N}.
   Context (G : grammar Σ N) `{acyclic G}.
 
   (* sat model *)
@@ -427,7 +427,7 @@ Section encoding.
       case_bool_decide; subst.
       * eapply reachable_from_left; eauto.
         rewrite app_nil_r. apply IHB.
-        2: by rewrite Nat.add_0_r in H3.
+        2: by rewrite Nat.add_0_r in H4.
         eapply succ_left; eauto.
       * eapply reachable_from_left; eauto.
         2: eapply Φ_derive_spec; eauto; lia.
@@ -633,8 +633,8 @@ Section encoding.
       * simpl. intros Heq. subst. rewrite Heq in Hψ2.
         eapply unary_clause_predicate_unique in Hψ1; [|exact Hψ2].
         congruence.
-      * simpl. intros [Heq1 [Heq2 ?]]. subst. rewrite Heq1 Heq2 in H2.
-        eapply binary_clause_predicate_unique in H2; [|exact H3].
+      * simpl. intros [Heq1 [Heq2 ?]]. subst. rewrite Heq1 Heq2 in H3.
+        eapply binary_clause_predicate_unique in H3; [|exact H4].
         have Heq : slice (decode m k) x n4 = slice (decode m k) x n1 by congruence.
         apply slice_eq_inv in Heq => //. 2-3: rewrite decode_length; lia.
         congruence.
